src/impl/TLS13.Impl.ConnectionState.LocalHandshake.fsti
@@ -67,6 +67,26 @@ fn try_start_handshake
            else
              connection_exactly c st0)
 
+fn try_start_server
+  (c:connection_state)
+  (#st0:erased CS.connection_state)
+  requires connection_exactly c st0 **
+           pure (Some? st0.CS.cs_model.CS.model_config.CS.config_server)
+  returns ok: bool
+  ensures (if ok then
+            connection_exactly c (started_server_state st0) **
+            pure (can_start_server st0 /\
+                  CS.legal_connection_delta
+                    st0
+                    {
+                      CS.delta_event = CS.ConnLocalEvent CS.LocalStartServer;
+                      CS.delta_raw_sent = B.empty;
+                      CS.delta_raw_received = B.empty;
+                    }
+                    (started_server_state st0))
+           else
+            connection_exactly c st0)
+
 fn try_send_client_hello
   (c:connection_state)
   (network_out:array U8.t)
